src/Std/Tactic/BVDecide/LRAT/Internal/Checker.lean
@@ -6,18 +6,19 @@ Authors: Henrik Böving
 module
 
 prelude
-import Std.Tactic.BVDecide.LRAT.NewInternal.Add
-import Std.Tactic.BVDecide.LRAT.NewInternal.Delete
-import Std.Tactic.BVDecide.LRAT.NewInternal.Rup
-import Std.Tactic.BVDecide.LRAT.NewInternal.Empty
+import Std.Tactic.BVDecide.LRAT.Internal.Add
+import Std.Tactic.BVDecide.LRAT.Internal.Delete
+import Std.Tactic.BVDecide.LRAT.Internal.Rup
+import Std.Tactic.BVDecide.LRAT.Internal.Empty
+import Std.Tactic.BVDecide.LRAT.Internal.Rat
 public import Std.Tactic.BVDecide.LRAT.Actions
 import Init.Omega
 
-namespace Std.Tactic.BVDecide.LRAT.NewInternal
+namespace Std.Tactic.BVDecide.LRAT.Internal
 
 open Std.Sat
 
-public def check (formula : CNF Nat) (proof : Array IntAction) : Bool :=
+public def check (proof : Array IntAction) (formula : CNF Nat) : Bool :=
   let state := .ofCNF formula
   go state proof 0
 where
@@ -32,7 +33,12 @@ where
           go (state.add clause) proof (idx + 1)
         else
           false
-      | .addRat .. => false -- TODO
+      | .addRat id clause pivot rupHints ratHints =>
+        let clause := convertClause clause
+        if state.checkRat clause pivot rupHints ratHints then
+          go (state.add clause) proof (idx + 1)
+        else
+          false
       | .del ids => go (state.deleteMany ids) proof (idx + 1)
     else
       false
@@ -60,17 +66,23 @@ theorem unsat_of_go {state : State} {proof : Array IntAction} {idx : Nat}
     apply State.entails_clause_of_checkRup
     exact h2
   case case3 => contradiction
-  case case4 => contradiction
-  case case5 ih =>
+  case case4 h2 ih =>
+    specialize ih h
+    apply CNF.unsat_of_forall_exists
+    intro a ha
+    apply State.unsat_of_unsat_of_checkRat h2 ha
+    exact ih
+  case case5 => contradiction
+  case case6 ih =>
     specialize ih h
     apply CNF.unsat_of_entails_unsat (h1 := ih)
     apply State.entails_deleteMany
-  case case6 => contradiction
+  case case7 => contradiction
 
-public theorem unsat_of_check {formula : CNF Nat} {proof : Array IntAction}
-    (h : check formula proof) : CNF.Unsat formula := by
+public theorem unsat_of_check {proof : Array IntAction} {formula : CNF Nat}
+    (h : check proof formula) : CNF.Unsat formula := by
   simp only [check] at h
   replace h := unsat_of_go h
   simpa using h
 
-end Std.Tactic.BVDecide.LRAT.NewInternal
+end Std.Tactic.BVDecide.LRAT.Internal
