src/Std/Sat/CNF/Unit.lean
@@ -7,6 +7,7 @@ module
 
 prelude
 public import Std.Sat.CNF.Basic
+public import Std.Sat.CNF.Sat
 public import Std.Sat.CNF.Relabel
 public import Std.Sat.CNF.Entails
 import Init.ByCases
